HittingSetToSetCover/HittingSetToSetCover_types.dfy
@@ -1,109 +1,309 @@
 include "../Problems/HittingSet.dfy"
 include "../Problems/SetCover.dfy"
-include "../Auxiliary/Set.dfy"
+include "../Reductions/ReductionHittingSetToSetCover.dfy"
+include "../Auxiliary/Lemmas.dfy"
 
 
-method HittingSet_to_SetCover_Method(U: Set<int>, S: SetSet<int>, k: nat) returns (r:(SetSet<int>, SetSetSet<int>, int), ghost counter:nat)
-  requires forall s | s in S.Model() ::  s <= U.Model() 
-  requires U.Model() == U.Universe()
-  requires S.Model() == S.Universe()
-  //ensures forall s | s in r.1 :: s <= r.0
-  //ensures isCover(r.0, r.1)
-  {
-    counter := 0;
-    //var newS: set<set<set<int>>> := (set u | u in U :: (set s | s in S && u in s));
-    var newS:SetSetSet<int>; newS, counter := NewSetSetSet(counter);
-    var U'; U', counter := U.Copy(counter);
-    var U'_empty:bool; U'_empty, counter := U'.Empty(counter);
+method HittingSet_to_SetCover_Method(U:Set<int>, S:SetSet<int>, k: nat) returns (r:(SetSet<int>, SetSetSet<int>, nat), ghost counter:nat)
+  //requires forall s | s in S ::  s <= U
+  //ensures r == HittingSet_to_SetCover(U, S, k) (en simple tampoco está puesto)
+  //ensures counter <= poly(U, S, k)
+  requires init_Set(U)
+  requires init_SetSet(S)
+  requires S.maximumSizeElements() <= U.Size()
+{
+  counter := 0;
 
-    assert counter <= U.Size() + 2;
-    ghost var counter_outer := counter;
-    while (!U'_empty)
-      decreases |U'.Model()|
-      invariant U'_empty == (U'.Model() == {})
-    {
-      ghost var U'_aux := U'.Model();
-      ghost var counter_outer_aux := counter;
-
-      var u:int; u, counter := U'.Pick(counter);
-      U', counter := U'.Remove(u, counter);
-
-      var sets_in_S_that_contain_u:SetSet<int>; sets_in_S_that_contain_u, counter := NewSetSet_params(S.Model(), S.maximumSizeElements(), counter);
-      var S':SetSet<int>; S', counter := S.Copy(counter);
-
-      var S'_empty:bool; S'_empty, counter := S'.Empty(counter);
-      //assert counter <= 1 + U.Size() + 1 + S.Size() + 1;
-
-      ghost var counter_inner := counter;
-      while (!S'_empty)
-        decreases |S'.Model()|
-        invariant S'_empty == (S'.Model() == {})
-        invariant correct_SetSet(S')
-        invariant correct_SetSet(sets_in_S_that_contain_u)
-        invariant in_universe_SetSet(S', S)
-        invariant in_universe_SetSet(sets_in_S_that_contain_u, S)
-        invariant counter <= counter_inner + (2*S.maximumSizeElements() + 2*S.Size() + 1)*(|S.Model()| - |S'.Model()|)
-      {
-        ghost var S'_aux := S'.Model();
-        ghost var counter_inner_aux := counter;
-
-        var s:Set<int>; s, counter := S'.Pick(counter);
-        S', counter := S'.Remove(s, counter);
-
-        //if (u in s) {
-        //  sets_in_S_that_contain_u := sets_in_S_that_contain_u + {s};
-        //}
-        var s_contains_u:bool; s_contains_u, counter := s.Contains(u, counter);
-        if (s_contains_u) {
-          sets_in_S_that_contain_u, counter := sets_in_S_that_contain_u.Add(s, counter);
-        }
-        //assert counter <= (counter_inner + S.maximumSizeElements() + S.Size() + S.maximumSizeElements() + sets_in_S_that_contain_u.Size());
-        //assert sets_in_S_that_contain_u.maximumSizeElements() == S.maximumSizeElements();
-        //assert sets_in_S_that_contain_u.Size() <= S.maximumSizeElements();
-
-        S'_empty, counter := S'.Empty(counter);
-        assume false;
-        assert counter <= counter_inner_aux + (2*S.maximumSizeElements() + 2*S.Size() + 1);
-        assert |S'_aux| - 1 == |S'.Model()|;
-        assert counter <= counter_inner + (2*S.maximumSizeElements() + 2*S.Size() + 1)*(|S.Model()| - |S'.Model()|);
-      }
-      
-      newS, counter := newS.Add(sets_in_S_that_contain_u, counter);
-      
-      U'_empty, counter := U'.Empty(counter);
-    }
-    //assert newS == (set u | u in U :: (set s | s in S && u in s));
-
-    assume false;
+  var newS:SetSetSet<int>; newS, counter := NewSetSetSet(counter);
+  var U':Set<int>; U', counter := U.Copy(counter);
+  var U'_empty:bool; U'_empty, counter := U'.Empty(counter);
+  assume false;
+  while (!U'_empty)
     /*
-    if ({} in S) then (S, (set s | s in S :: {s}), 0)
-    else
-    tisCover(U,S);
-    (S, newS, k)
+    decreases |U'|
+    invariant U' <= U
+    invariant newS == (set u | u in (U - U') :: (set s | s in S && u in s))
+    invariant counter <= 1 + |U| + (|U| - |U'|)*(poly_outer_loop(U, S, k) + 1)
     */
-    var empty_set:Set<int>; empty_set, counter := NewSet(counter);
-    var S_contains_empty:bool; S_contains_empty, counter := S.Contains(empty_set, counter);
-    if (S_contains_empty) {
-      
-      var S':SetSet<int>; S', counter := S.Copy(counter);
-      var S'_empty:bool; S'_empty, counter := S'.Empty(counter);
-      while (!S'_empty) {
-        var s:Set<int>; s, counter := S'.Pick(counter);
-        S', counter := S'.Remove(s, counter);
+    // Termination
+    decreases U'.Cardinality()
+    // Types
 
-        var set_of_s:SetSet<int>; set_of_s, counter := NewSetSet<int>(counter);
-        set_of_s, counter := set_of_s.Add(s, counter);
+    // Regular invariants
 
-        newS, counter := newS.Add(set_of_s, counter);
-        S'_empty, counter := S'.Empty(counter);
-      }
+    // Counter
 
-      return (S, newS, 0), counter;
-      
-    }
-    else {
-      return (S, newS, k), counter;
-    }
-
+  {
+    U', newS, U'_empty, counter := HittingSet_to_SetCover_outer_loop(U, S, k, U', newS, counter);
+  }
+  /*
+  identity_substraction_lemma(U.Model(), U'.Model());
+  var S_contains_empty:bool := false;
+  var S' := S; counter := counter + |S|*|U|;
+  assert counter <= poly_aux_1(U, S, k);
+  while (S' != {})
+    decreases |S'|
+    invariant S' <= S
+    invariant S_contains_empty == ({} in (S - S'))
+    invariant counter <= poly_aux_1(U, S, k) + (|S| - |S'|)*(poly_contains_empty_loop(U, S, k) + 1)
+  {
+    S', S_contains_empty, counter := HittingSet_to_SetCover_S_contains_empty_loop(U, S, k, S', S_contains_empty, counter);
   }
 
+  if (S_contains_empty) {
+    var newS := {};
+    var S' := S;
+    assert counter <= poly_aux_2(U, S, k);
+    while (S' != {})
+      decreases |S'|
+      invariant S' <= S
+      invariant newS == (set s | s in (S - S') :: {s})
+      invariant counter <= poly_aux_2(U, S, k) + (|S| - |S'|)*(poly_edge_case_loop(U, S, k) + 1)
+    {
+      S', newS, counter := HittingSet_to_SetCover_edge_case_loop(U, S, k, S', newS, counter);
+    }
+    assert counter <= poly(U, S, k);
+    return (S, newS, 0), counter;
+  }
+  else {
+    return (S, newS, k), counter;
+  }
+  */
+}
+
+
+method HittingSet_to_SetCover_outer_loop(U:Set<int>, S:SetSet<int>, k:nat, U':Set<int>, newS:SetSetSet<int>, ghost counter_in:nat) returns (U'':Set<int>, newS':SetSetSet<int>, U''_empty:bool, ghost counter:nat)
+// Termination in
+requires U'.Model() != {}
+// Types in
+requires S.Valid()
+requires newS.Valid()
+requires in_universe_Set(U', U)
+requires S.maximumSizeElements() <= U.Size()
+// Invariant in
+requires forall s | s in S.Model() ::  s <= U.Model()
+requires newS.Model() == (set u | u in (U.Model() - U'.Model()) :: (set s | s in S.Model() && u in s))
+// Termination out
+ensures U''.Cardinality() == U'.Cardinality() - 1
+ensures U''_empty == (U''.Model() == {})
+// Types out
+ensures newS'.Valid()
+ensures in_universe_Set(U'', U)
+// Invariant out
+ensures newS'.Model() == (set u | u in (U.Model() - U''.Model()) :: (set s | s in S.Model() && u in s))
+// Counter
+//ensures counter <= counter_in + poly_outer_loop(U, S, k)
+{
+  counter := counter_in;
+  var u:int; u, counter := U'.Pick(counter);
+  U'', counter := U'.Remove(u, counter);
+
+  var sets_in_S_that_contain_u:SetSet<int>; sets_in_S_that_contain_u, counter := NewSetSet_params(S.Model(), S.maximumSizeElements(), counter);
+  var S'; S', counter := S.Copy(counter);
+  var S'_empty; S'_empty, counter := S'.Empty(counter);
+  while (!S'_empty)
+    // Termination
+    decreases S'.Cardinality()
+    invariant S'_empty == (S'.Model() == {})
+    // Types
+    invariant U.Valid()
+    invariant in_universe_SetSet(S', S)
+    invariant in_universe_SetSet(sets_in_S_that_contain_u, S)
+    invariant S.maximumSizeElements() <= U.Size()
+    // Regular invariants
+    invariant forall s | s in S.Model() ::  s <= U.Model()
+    invariant sets_in_S_that_contain_u.Model() == (set s | s in (S.Model() - S'.Model()) && u in s)
+    // Counter
+
+  {
+    S', sets_in_S_that_contain_u, S'_empty, counter := HittingSet_to_SetCover_middle_loop(U, S, k, S', u, sets_in_S_that_contain_u, counter);
+  }
+  newS', counter := newS.Add(sets_in_S_that_contain_u, counter);
+  U''_empty, counter := U''.Empty(counter);
+
+  assert newS'.Model() == (set v | v in (U.Model() - U''.Model()) :: (set s | s in S.Model() && v in s)) by {
+    assert newS'.Model() == (set v | v in (U.Model() - U'.Model()) :: (set s | s in S.Model() && v in s)) + {sets_in_S_that_contain_u.Model()};
+    assert newS'.Model() == (set v | v in (U.Model() - U'.Model()) :: (set s | s in S.Model() && v in s)) + {(set s | s in (S.Model() - S'.Model()) && u in s)};
+    assert (S.Model() - S'.Model()) == S.Model();
+    assert newS'.Model() == (set v | v in (U.Model() - U'.Model()) + {u} :: (set s | s in S.Model() && v in s));
+    assert (U.Model() - U''.Model()) == (U.Model() - U'.Model()) + {u};
+  }
+}
+
+
+
+method HittingSet_to_SetCover_middle_loop(U:Set<int>, S:SetSet<int>, k:nat, S':SetSet<int>, u:int, sets_in_S_that_contain_u:SetSet<int>, ghost counter_in:nat) returns (S'':SetSet<int>, sets_in_S_that_contain_u':SetSet<int>, S''_empty:bool, ghost counter:nat)
+// Termination in
+requires S'.Model() != {}
+// Types in
+requires U.Valid()
+requires in_universe_SetSet(S', S)
+requires in_universe_SetSet(sets_in_S_that_contain_u, S)
+requires S.maximumSizeElements() <= U.Size()
+// Invariant in
+requires forall s | s in S.Model() ::  s <= U.Model()
+requires sets_in_S_that_contain_u.Model() == (set s | s in (S.Model() - S'.Model()) && u in s)
+// Termination out
+ensures S''.Cardinality() == S'.Cardinality() - 1
+ensures S''_empty == (S''.Model() == {})
+// Types out
+ensures in_universe_SetSet(S'', S)
+ensures in_universe_SetSet(sets_in_S_that_contain_u', S)
+// Invariant out
+ensures sets_in_S_that_contain_u'.Model() == (set s | s in (S.Model() - S''.Model()) && u in s)
+// Counter
+ensures counter <= counter_in + poly_middle_loop(U, S, k)
+{
+  in_universe_lemma_SetSet(S', S);
+  in_universe_lemma_SetSet(sets_in_S_that_contain_u, S);
+  counter := counter_in;
+  sets_in_S_that_contain_u', counter := sets_in_S_that_contain_u.Copy(counter);
+
+  var s:Set<int>; s, counter := S'.Pick(counter);
+  S'', counter := S'.Remove(s, counter);
+
+  var s_contains_u:bool := false;
+  var s':Set<int>; s', counter := s.Copy(counter);
+  var s'_empty:bool; s'_empty, counter := s'.Empty(counter);
+  while (!s'_empty)
+    // Termination
+    decreases s'.Cardinality()
+    invariant s'_empty == (s'.Model() == {})
+    // Types
+    invariant s'.Valid()
+    invariant in_universe_Set(s', s)
+    invariant s.Cardinality() <= S.maximumSizeElements()
+    invariant S.maximumSizeElements() <= U.Size()
+    // Regular invariants
+    invariant s_contains_u == (u in (s.Model() - s'.Model()))
+    // Counter
+    invariant counter <= counter_in + 2*S.Size() + 2*U.Size() + constant + (s.Cardinality() - s'.Cardinality())*poly_inner_loop(U, S, k)
+  {
+    s', s_contains_u, s'_empty, counter := HittingSet_to_SetCover_inner_loop(U, S, k, s, s', u, s_contains_u, counter);
+  }
+  mult_preserves_order(s.Cardinality(), poly_inner_loop(U, S, k), U.Size(), poly_inner_loop(U, S, k));
+  if (s_contains_u) {
+    sets_in_S_that_contain_u', counter := sets_in_S_that_contain_u.Add(s, counter);
+  }
+  S''_empty, counter := S''.Empty(counter);
+  assert counter <= counter_in + 3*S.Size() + 2*U.Size() + 2*constant + U.Size()*poly_inner_loop(U, S, k);
+}
+
+method HittingSet_to_SetCover_inner_loop(U:Set<int>, S:SetSet<int>, k:nat, s:Set<int>, s':Set<int>, u:int, s_contains_u:bool, ghost counter_in:nat) returns (s'':Set<int>, s_contains_u':bool, s''_empty:bool, ghost counter:nat)
+// Termination in
+requires s'.Model() != {}
+// Types in
+requires U.Valid()
+requires S.Valid()
+requires in_universe_Set(s', s)
+requires s.Cardinality() <= S.maximumSizeElements()
+requires S.maximumSizeElements() <= U.Size()
+// Invariant in
+requires s_contains_u == (u in (s.Model() - s'.Model()))
+// Termination out
+ensures s''.Cardinality() == s'.Cardinality() - 1
+ensures s''_empty == (s''.Model() == {})
+// Types out
+ensures s''.Valid()
+ensures in_universe_Set(s'', s)
+// Invariant out
+ensures s_contains_u' == (u in (s.Model() - s''.Model()))
+// Counter
+ensures counter <= counter_in + poly_inner_loop(U, S, k)
+{
+  if_smaller_then_less_cardinality(s'.Universe(), s.Model());
+  counter := counter_in;
+  s_contains_u' := s_contains_u;
+  var e:int; e, counter := s'.Pick(counter);
+  s'', counter := s'.Remove(e, counter);
+  if (e == u) {
+    s_contains_u' := true;
+  }
+  s''_empty, counter := s''.Empty(counter);
+}
+
+method HittingSet_to_SetCover_S_contains_empty_loop(U:Set<int>, S:SetSet<int>, k:nat, S':SetSet<int>, S_contains_empty:bool, ghost counter_in:nat) returns (S'':SetSet<int>, S_contains_empty':bool, ghost counter:nat)
+// Termination in
+requires S'.Model() != {}
+// Types in
+requires U.Valid()
+requires in_universe_SetSet(S', S)
+requires S.maximumSizeElements() <= U.Size()
+// Invariant in
+requires S_contains_empty == ({} in (S.Model() - S'.Model()))
+// Termination out
+ensures S''.Cardinality() == S'.Cardinality() - 1
+// Types out
+ensures in_universe_SetSet(S'', S)
+ensures S''.maximumSizeElements() <= U.Size()
+// Invariant out
+ensures S_contains_empty'== ({} in (S.Model() - S''.Model()))
+// Counter
+ensures counter <= counter_in + poly_contains_empty_loop(U, S, k)
+{
+  in_universe_lemma_SetSet(S', S);
+  counter := counter_in;
+  var s:Set<int>; s, counter := S'.Pick(counter);
+  S'', counter := S'.Remove(s, counter);
+  var s_empty:bool; s_empty, counter := s.Empty(counter);
+  S_contains_empty' := S_contains_empty || s_empty;
+}
+
+method HittingSet_to_SetCover_edge_case_loop(U:Set<int>, S:SetSet<int>, k:nat, S':SetSet<int>, newS:SetSetSet<int>, ghost counter_in:nat) returns (S'':SetSet<int>, newS':SetSetSet<int>, ghost counter:nat)
+// Termination in
+requires S'.Model() != {}
+// Types in
+requires U.Valid()
+requires newS.Valid()
+requires in_universe_SetSet(S', S)
+requires S.maximumSizeElements() <= U.Size()
+// Invariant in
+requires newS.Model() == (set s | s in (S.Model() - S'.Model()) :: {s})
+requires newS.Cardinality() <= S.Cardinality() - S'.Cardinality()
+requires newS.maximumSizeElements() <= S.maximumSizeElements()
+// Termination out
+ensures S''.Cardinality() == S'.Cardinality() - 1
+// Types out
+ensures newS'.Valid()
+ensures in_universe_SetSet(S'', S)
+// Invariant out
+ensures newS'.Model() == (set s | s in (S.Model() - S''.Model()) :: {s})
+ensures newS'.Cardinality() <= S.Cardinality() - S''.Cardinality()
+ensures newS'.maximumSizeElements() <= S.maximumSizeElements()
+// Counter
+ensures counter <= counter_in + poly_edge_case_loop(U, S, k)
+{
+  in_universe_lemma_SetSet(S', S);
+  mult_preserves_order(newS.Cardinality(), newS.maximumSizeElements(), S.Cardinality(), S.maximumSizeElements());
+  counter := counter_in;
+  var s:Set<int>; s, counter := S'.Pick(counter);
+  S'', counter := S'.Remove(s, counter);
+  var s_set:SetSet<int>; s_set, counter := NewSetSet(counter);
+  s_set, counter := s_set.Add(s, counter);
+  newS', counter := newS.Add(s_set, counter);
+}
+
+
+ghost function poly_inner_loop(U: Set<int>, S: SetSet<int>, k: nat) : (o:nat)
+{
+  U.Size() + 2*constant
+}
+ghost function poly_middle_loop(U: Set<int>, S: SetSet<int>, k: nat) : (o:nat)
+  ensures 3*S.Size() + 2*U.Size() + 2*constant + U.Size()*poly_inner_loop(U, S, k) <= o
+{
+  /*calc <= {
+    3*S.Size() + 2*U.Size() + 2*constant + U.Size()*poly_inner_loop(U, S, k);
+    3*S.Size() + 2*U.Size() + 2*constant + U.Size()*(U.Size() + 2*constant);
+    3*S.Size() + 2*U.Size() + 2*constant + U.Size()*U.Size() + 2*U.Size();
+    U.Size()*U.Size() + 3*S.Size() + 4*U.Size() + constant;
+  }*/
+  U.Size()*U.Size() + 3*S.Size() + 4*U.Size() + 2*constant
+}
+ghost function poly_contains_empty_loop(U: Set<int>, S: SetSet<int>, k: nat) : (o:nat)
+{
+  S.Size() + U.Size() + constant
+}
+ghost function poly_edge_case_loop(U: Set<int>, S: SetSet<int>, k: nat) : (o:nat)
+{
+  2*S.Size() + 2*U.Size() + constant
+}
