VerificationSetCover/VerificationSetCover_simple.dfy
@@ -9,8 +9,7 @@ ensures b == (I <= S && isCover(U, I) && |I| <= k)
 ensures counter <= poly(U, S, k, I)
 {
   counter := 0;
-  var U' := U;
-  counter := counter + |U|;
+  var U' := U; counter := counter + |U|;
   b:= true;
   var I_seq_S:bool;
   I_seq_S, counter := isSubset(U, I, S, counter);
@@ -42,8 +41,7 @@ ensures counter <= counter_in + poly_isSubset(U, S1, S2)
 {
   counter := counter_in;
   b := true;
-  var S1':= S1;
-  counter := counter + |U|*|S1|;
+  var S1':= S1; counter := counter + |U|*|S1|;
   while (S1' != {})
   // Termination
   decreases |S1'|
@@ -53,9 +51,10 @@ ensures counter <= counter_in + poly_isSubset(U, S1, S2)
   // Counter
   invariant counter <= counter_in + |S1|*|U| + constant + (|S1| - |S1'|)*(poly_isSubset_loop(U, S1, S2) + 1)
   {
-    S1', b, counter := isSubset_loop(U, S1, S2, S1', counter, b);
     counter := counter + 1;
+    S1', b, counter := isSubset_loop(U, S1, S2, S1', counter, b);
   }
+  counter := counter + 1;
 }
 
 method isSubset_loop(U:set<int>, S1:set<set<int>>, S2:set<set<int>>, S1':set<set<int>>, ghost counter_in:nat, b:bool) returns (S1'':set<set<int>>, b':bool, ghost counter:nat)
@@ -72,14 +71,11 @@ ensures S1'' <= S1
 // Counter
 ensures counter <= counter_in + poly_isSubset_loop(U, S1, S2)
 {
-  if_smaller_then_less_cardinality(S1', S1);
   counter := counter_in;
-  var s:set<int> :| s in S1';
-  counter := counter + |U|;
-  b' := b && s in S2;
-  counter := counter + |S2|*|U|;
-  S1'' := S1' - {s};
-  counter := counter + |S1|*|U|;
+  if_smaller_then_less_cardinality(S1', S1);
+  var s:set<int> :| s in S1'; counter := counter + |U|;
+  b' := b && s in S2; counter := counter + |S2|*|U|;
+  S1'' := S1' - {s}; counter := counter + |S1|*|U|;
 }
 
 
@@ -98,13 +94,11 @@ ensures b1 == isCover(U - U'', I)
 ensures counter <= counter_in + poly_outer_loop(U, S, k, I)
 {
   counter := counter_in;
-  var u :| u in U';
-  counter := counter + 1;
-  U'' := U' - {u};
-  counter := counter + |U|;
+  var u :| u in U'; counter := counter + 1;
+  U'' := U' - {u}; counter := counter + |U|;
 
-  var I' := I; var b2:= false;
-  counter := counter + |S|*|U|;
+  var I' := I; counter := counter + |S|*|U|;
+  var b2:= false;
   while (I' != {} && !b2)
     decreases |I'|
     invariant I' <= I
@@ -135,12 +129,9 @@ ensures b2 == (exists i' | i' in I - I'' :: u in i')
 ensures counter == counter_in + poly_inner_loop(U, S, k)
 {
   counter := counter_in;
-  var i :| i in I';
-  counter := counter + |U|;
-  b2 := u in i;
-  counter := counter + |U|;
-  I'' := I' - {i};
-  counter := counter + |S|*|U|;
+  var i :| i in I'; counter := counter + |U|;
+  b2 := u in i; counter := counter + |U|;
+  I'' := I' - {i}; counter := counter + |S|*|U|;
 }
 
 lemma counter_simplification(U:set<int>, S:set<set<int>>, k:nat, I:set<set<int>>, U':set<int>)
@@ -152,11 +143,11 @@ ensures |U| + poly_isSubset(U, I, S) + 2 + (|U| - |U'|)*(poly_outer_loop(U, S, k
   calc <= {
     |U| + poly_isSubset(U, I, S) + 2 + (|U| - |U'|)*(poly_outer_loop(U, S, k, I) + 1);
     |U| + poly_isSubset(U, I, S) + 2 + |U|*poly_outer_loop(U, S, k, I) + |U|;
-    |U| + |I|*|I|*|U| + |I|*|S|*|U| + 2*|I|*|U| + |I| + constant + 2 + |U|*poly_outer_loop(U, S, k, I) + |U|;
-    |I|*|I|*|U| + |I|*|S|*|U| + 2*|I|*|U| + |I| + 2*|U| + 3 + |U|*poly_outer_loop(U, S, k, I);
-    |I|*|I|*|U| + |I|*|S|*|U| + 2*|I|*|U| + |I| + 2*|U| + 3 + |U|*(|I|*|S|*|U| + 2*|I|*|U| + |S|*|U| + |I| + |U| + 2);
-    |I|*|I|*|U| + |I|*|S|*|U| + 2*|I|*|U| + |I| + 2*|U| + 3 + |I|*|S|*|U|*|U| + 2*|I|*|U|*|U| + |S|*|U|*|U| + |I|*|U| + |U|*|U| + 2*|U|;
-    |I|*|S|*|U|*|U| + |I|*|I|*|U| + |I|*|S|*|U| + 2*|I|*|U|*|U| + |S|*|U|*|U| + 3*|I|*|U| + |U|*|U| + |I| + 4*|U| + 3;
+    |U| + |I|*|I|*|U| + |I|*|S|*|U| + 2*|I|*|U| + |I| + 4 + |U|*poly_outer_loop(U, S, k, I) + |U|;
+    |I|*|I|*|U| + |I|*|S|*|U| + 2*|I|*|U| + |I| + 2*|U| + 4 + |U|*poly_outer_loop(U, S, k, I);
+    |I|*|I|*|U| + |I|*|S|*|U| + 2*|I|*|U| + |I| + 2*|U| + 4 + |U|*(|I|*|S|*|U| + 2*|I|*|U| + |S|*|U| + |I| + |U| + 2);
+    |I|*|I|*|U| + |I|*|S|*|U| + 2*|I|*|U| + |I| + 2*|U| + 4 + |I|*|S|*|U|*|U| + 2*|I|*|U|*|U| + |S|*|U|*|U| + |I|*|U| + |U|*|U| + 2*|U|;
+    |I|*|S|*|U|*|U| + |I|*|I|*|U| + |I|*|S|*|U| + 2*|I|*|U|*|U| + |S|*|U|*|U| + 3*|I|*|U| + |U|*|U| + |I| + 4*|U| + 4;
   }
 }
 
@@ -166,7 +157,7 @@ ghost function poly_isSubset_loop(U: set<int>, S1:set<set<int>>, S2:set<set<int>
 }
 ghost function poly_isSubset(U: set<int>, S1:set<set<int>>, S2:set<set<int>>) : (o:nat)
 {
-  |S1|*|S1|*|U| + |S1|*|S2|*|U| + 2*|S1|*|U| + |S1| + 1
+  |S1|*|S1|*|U| + |S1|*|S2|*|U| + 2*|S1|*|U| + |S1| + 2
 }
 ghost function poly_inner_loop(U: set<int>, S: set<set<int>>, k: nat) : (o:nat) {
   |S|*|U| + 2*|U|
@@ -178,5 +169,5 @@ ensures |S|*|U| + |U| + 2 + |I|*(|S|*|U| + 2*|U| + 1) == o
 }
 
 ghost function poly(U: set<int>, S: set<set<int>>, k: nat, I:set<set<int>>) : (o:nat) {
-  |I|*|S|*|U|*|U| + |I|*|I|*|U| + |I|*|S|*|U| + 2*|I|*|U|*|U| + |S|*|U|*|U| + 3*|I|*|U| + |U|*|U| + |I| + 4*|U| + 3
+  |I|*|S|*|U|*|U| + |I|*|I|*|U| + |I|*|S|*|U| + 2*|I|*|U|*|U| + |S|*|U|*|U| + 3*|I|*|U| + |U|*|U| + |I| + 4*|U| + 4
 }
